theories/lang_oadt/progress.v
@@ -3,13 +3,10 @@ From oadt Require Import lang_oadt.syntax.
 From oadt Require Import lang_oadt.semantics.
 From oadt Require Import lang_oadt.typing.
 From oadt Require Import lang_oadt.infrastructure.
-From oadt Require Import lang_oadt.properties.
+From oadt Require Import lang_oadt.values.
 From oadt Require Import lang_oadt.admissible.
 From oadt Require Import lang_oadt.inversion.
 From oadt Require Import lang_oadt.equivalence.
-
-(** * Progress *)
-(** The progress metatheorem. *)
 
 Import syntax.notations.
 Import semantics.notations.
@@ -25,7 +22,9 @@ Section progress.
 Context (Σ : gctx).
 Context (Hwf : gctx_wf Σ).
 
-(** ** Canonical forms *)
+Set Default Proof Using "Hwf".
+
+(** * Canonical forms *)
 Ltac canonical_form_solver :=
   inversion 1; intros; subst; eauto;
   apply_type_inv;
@@ -108,9 +107,9 @@ Proof.
 Qed.
 
 
-(** ** Progress *)
+(** * Progress *)
 
-(** Take a step through evaluation context. *)
+(** Dealing with evaluation context. *)
 Ltac step_ectx_solver :=
   match goal with
   | H : _ ⊨ _ -->! _ |- exists _, _ ⊨ _ -->! _ =>
